---
title: Solving the general Fibonacci Sequence
description: Finding a iterative solution to a general Fibonacci Sequence
tags: [maths, number]
banner: thoughts.jpg
---

This is a question where I was given the solution sometime in high school, but
had forgotten about over the years. Given that I have an ample amount of free
time, I thought I might give this question a tackle for the sake of keeping my
mind active.

## Defining the problem

The [Fibonacci sequence](https://en.wikipedia.org/wiki/Fibonacci_number)
$\lbrace 1,1,2,3,5,8,13\ldots\rbrace$, with the [recurrence
relation](https://en.wikipedia.org/wiki/Recurrence_relation) $F_n = F_{n-1} +
F_{n-2}$ is famously known for generating the [Golden
ratio](https://en.wikipedia.org/wiki/Golden_ratio) $\phi = (\sqrt{5}+1)/2$.

But the generation of the golden ratio is not unique to this particular
starting point of the Fibonacci sequence. In fact, even if you decide to start
out with different first and second terms, the Golden ratio still appears in
the generated integers.

It should be that the result of having the Golden ratio appear is more related
to the recurrence relation itself rather than the specific sequence itself.
With a different recurrence relation, we should expect different ratios to
appear in the resulting sequence.

So our generalized question is as followed: Given the recurrence relation

$$
x_n = a x_{n-1} + b x_{n-2} ; \;n \geq 2
$$

Can we find the closed-form expression of $x_n$?

## The general strategy

We attempt to require the recurrence relation into one that we already know how
to solve: a simple geometric sequence. In particular, we attempt to find $y_n =
x_n + g x_{n-1}$ so that we can write the recurrence relation as a geometric
sequence of $y_n$ : $y_n = \alpha y_{n-1}$

Explicitly writing this out in terms of the original recurrence relation:

$$
x_n + g x_{n-1} = (a + g) x_{n-1} + b x_{n-2} \\
x_n + g x_{n-1} = (a + g) \enc{x_{n-1} + \frac{b}{a+g} x_{n-2}} \\
$$

For the second equation to be a simple geometric sequence, we can see that $g$
is restricted to the root of the equation:

$$
g = \frac{b}{a+g} \; \rightarrow \; g^2 + a g - b = 0
$$

The coefficients in the original recurrence relations define a characteristic
equation for $g$. Here we need to take into account that the characteristic
equation could have repeated roots. But let's first tackle the one without
repeated roots first.

## Solution with unique roots

Given the two roots $g_1$, $g_2$, we know have two geometric equation that
could be used to rewrite our original recurrent relation:

$$
y_n = x_n + g_1 x_{n-1} \; y_n = (a + g_1) y_{n-1} = \alpha y_{n-1} \\
z_n = x_n + g_2 x_{n-1} \; z_n = (a + g_2) z_{n-1} = \beta z_{n-1} \\
$$

The closed form of the sequence for $y_n$ and $z_n$ could then be written as:

$$
y_n = \alpha^{n} y_0 \;;\; z_n = \beta^n z_0
$$

It might feel a bit fishy writing $y_0 = x_{0} - x_{-1}$, but one can simply
view it as a continuation of the sequence in the negative direction while
keeping the recurrence relation. For example, in the case of the Fibonacci
sequence, we can include the negative terms into something like: $\lbrace
\ldots0,1,0,1,1,2,3,\ldots\rbrace$. Or, you can of course simple shift the
dependence on $n$ to be something like $y_n = \alpha^{n-1}y_1$. In any case,
you can think of $y_0$ and $z_0$ as constants determined by the initial terms
of the sequence, independent of the actual recurrence relation. After solving
the closed form of $y_n$ and $z_n$, we could solve $x_n$ using simple algebra
to eliminate the dependence for $x_{n-1}$:

$$
x_n = \frac{g_2 y_n - g_1 z_n}{g_2 - g_1} = \frac{g_2 (a + g_1)^{n-1}(x_{1} + g_1 x_{0}) - g_1(a+g_2)^{n-1}(x_{1} + g_2 x_{0})}{g_2 - g_1}
$$

In our special case of the Fibonacci sequence with $F_1=1$, $F_0=0$, $a=b=1$.
The characteristic equation is given as:

$$
g^2 + g - 1  = 0 \;\rightarrow \; g_{\pm} = \frac{-1\pm\sqrt{5}}{2} \;;\quad g_+ - g_- = \sqrt{5}
$$

Taking in these numbers into the general solution above, we get the relation:

$$
F_n = \frac{1}{\sqrt{5}}\left(\left(\frac{-1+\sqrt{5}}{2}\right)\left(\frac{1-\sqrt{5}}{2}\right)^{n-1} - \left(\frac{-1-\sqrt{5}}{2}\right)\left(\frac{1+\sqrt{5}}{2}\right)^{n-1} \right)
$$

or

$$
F_n = \frac{1}{\sqrt{5}}\left( \left(\frac{1+\sqrt{5}}{2}\right)^{n} - \left(\frac{1-\sqrt{5}}{2}\right)^{n}\right) \\
= \frac{1}{\sqrt{5}} \left( \phi^{n} - \varphi^{n} \right)
$$

Which is what we find on
[wikipedia](https://en.wikipedia.org/wiki/Fibonacci_number#Closed-form_expression)!
The relation here with the golden ratio is also make apparent in the closed
form, as $\lvert \phi\rvert > \lvert \varphi \rvert$, asymptotically the
Fibonacci sequence approaches a geometric sequence with a ratio of $\phi$.

# Solution with the repeated roots.

In the case that the coefficients in the recurrence relation satisfies the
relation: $b = -(a/2)^2 = -g_0^2$, then the characteristic equation has
repeated roots of $-g_0$, we are left with the single extended sequence:

$$
y_n = x_n - g_0 x_{n-1}\;;\; y_n = g_0 y_{n-1}
$$

the solution is to further decouple $x_n$ from $x_{n-1}$, after already knowing
that $y_n = g_0^n y_0$, is make the assumption that $x_{n} = g_0^{n} f(n)$,
then the relation between $y_n$ and $x_m$ could be rewritten as:

$$
g_0^n y_0 = g_0^n f(n) - g_0^n f(n-1) \;\rightarrow \; f(n) - f(n-1) = y_0.
$$

Again, $y_0$ is some constant to be determined by the initial terms of $x$. The
recurrence relation for $f(n)$ is such that it is at most an arithmetic
sequence, in other words: $f(n) = c_0 + n c_1$. So the closed form of $x_n$ is:

$$
x_n = g_0^n ( c_0 + n c_1 )
$$
